theories/Iris/Model.v
@@ -583,6 +583,15 @@ Module Type IrisResources
       by iApply semWP_call_frame.
     Qed.
 
+    Lemma semWP_call_inline {Γ τ Δ} (f : 𝑭 Δ τ) (es : NamedEnv (Exp Γ) Δ) :
+      ⊢ ∀ (Q : Val τ → CStore Γ → iProp Σ) (δΓ : CStore Γ),
+          semWP (FunDef f) (fun vτ _ => Q vτ δΓ) (evals es δΓ) -∗
+          semWP (stm_call f es) Q δΓ.
+    Proof.
+      iIntros (Q δΓ) "wpbody".
+      by iApply semWP_call_inline_later.
+    Qed.
+
     Lemma semWP_bind {Γ τ σ} (s : Stm Γ σ) (k : Val σ → Stm Γ τ) :
       ⊢ ∀ (Q : Val τ → CStore Γ → iProp Σ) (δ : CStore Γ),
           semWP s (fun v => semWP (k v) Q) δ -∗ semWP (stm_bind s k) Q δ.
@@ -759,6 +768,28 @@ Module Type IrisResources
       destruct eval.
       - by iApply (semWP_block [env].[xinl0∷σinl0 ↦ v]).
       - by iApply (semWP_block [env].[xinr0∷σinr0 ↦ v]).
+    Qed.
+
+    Lemma semWP_match_prod {Γ τ σ1 σ2 xl xr} (e : Exp Γ (ty.prod σ1 σ2)) (s : Stm (Γ ▻ xl∷σ1 ▻ xr∷σ2) τ) :
+      ⊢ ∀ (Q : Val τ → CStore Γ → iProp Σ) (δ : CStore Γ),
+          (let (v1, v2) := eval e δ in
+           semWP s (fun v δ1 => Q v (env.tail (env.tail δ1))) δ.[xl∷σ1 ↦ v1].[xr∷σ2 ↦ v2]) -∗
+          semWP (stm_match_prod e xl xr s) Q δ.
+    Proof.
+      iIntros (Q δ) "WPs". unfold semWP at 2. rewrite wp_unfold. cbn.
+      iIntros (σ _ ks1 ks nt) "Hregs".
+      iMod (fupd_mask_subseteq empty) as "Hclose"; first set_solver.
+      iModIntro. iSplitR; [trivial|].
+      iIntros (e2 σ' efs) "%".
+      dependent elimination H.
+      fold_semWP.
+      dependent elimination s0.
+      iModIntro. iModIntro. iModIntro.
+      iMod "Hclose" as "_".
+      iModIntro. iFrame.
+      iSplitL; [|trivial].
+      destruct eval.
+      by iApply (semWP_block [env].[_∷_ ↦ _].[_∷_ ↦ _]).
     Qed.
 
     Lemma semWP_match_enum {Γ τ E} (e : Exp Γ (ty.enum E)) (alts : enumt E → Stm Γ τ) :
